testdata/wild/rfc3339-offset-overrange/rfc3339-offset-overrange.cue
@@ -1,0 +1,2 @@
+import "time"
+x: time.Time & "2020-01-01T00:00:00+25:00"
